small change to fake

proof/equiv.py
@@ -9,8 +9,8 @@ regexEquiv = r"equiv \[(.*) ~ (.*) : (.*) ==> (.*)\]"
 regexLine = r"([^;{}]*;|[^;{}]* [{][^}]*[}])"
 
 m = match(regexEquiv, eq)
-print(m.group(3))
-print()
+#print(m.group(3))
+#print()
 m1 = findall(regexLine, m.group(1))
 m2 = findall(regexLine, m.group(2))
 n1 = len(m1)
@@ -22,5 +22,5 @@ else:
 size = str(min(80, max(map(len, m1))))
 for i in range(len(m1)):
   print(("{i:3}: {left:"+size+"} | {right}").format(i=i+1, left=m1[i], right=m2[i]))
-print()
-print(m.group(4))
+#print()
+#print(m.group(4))
